In~\cite{gregory2023iterated} the authors
propose the following conjecture for row sums of iterated rascal triangles.
\begin{conj}
    \label{conjecture:row_sums}
    (Conjecture 7.5 in~\cite{gregory2023iterated}.)
    For every $i$
    \begin{align*}
        \sum_{k=0}^{4i+3} \rascalNumber{4i+3}{k}{i} &= 2^{4i+2}
    \end{align*}
\end{conj}
\begin{proof}
    Rewrite conjecture statement explicitly as
    \begin{align*}
        \sum_{k=0}^{4i+3} \sum_{m=0}^{i} \binom{4i+3-k}{m} \binom{k}{m} = 2^{4i+2}
    \end{align*}
    Rearranging sums and omitting summation bounds yields
    \begin{equation}
        \sum_{m=0}^{i}  \sum_{k} \binom{4i+3-k}{m} \binom{k}{m} = 2^{4i+2}\label{eq:row_sums_conjecture_explicit}
    \end{equation}
    In Concrete mathematics [\cite{graham1994concrete}, p.\ 169, eq (5.26)], Knuth et al.
    provide the identity for the column sum of binomial coefficients multiplication
    \begin{equation}
        \label{eq:binomial_coefficients_column_sum}
        \sum_{k=0}^{l} \binom{l-k}{m} \binom{q+k}{n} = \binom{l+q+1}{m+n+1}
    \end{equation}
    We can observe this pattern in the equation~\eqref{eq:row_sums_conjecture_explicit},
    thus the sum $\sum_{k} \binom{4i+3-k}{m} \binom{k}{m}$ equals to
    \begin{align*}
        \sum_{k} \binom{4i+3-k}{m} \binom{k}{m} = \binom{4i+4}{2m+1}
    \end{align*}
    Therefore, conjecture~\eqref{conjecture:row_sums} is equivalent to
    \begin{align*}
        \sum_{m=0}^{i} \binom{4i+4}{2m+1} = 2^{4i+2}
    \end{align*}
    Note that
    \begin{align*}
        \sum_{m=0}^{2i+1} \binom{4i+4}{2m+1} = 2^{4i+3}
    \end{align*}
    So that
    \begin{align*}
        \sum_{m=0}^{\frac{2i+1}{2}} \binom{4i+4}{2m+1} = \sum_{m=0}^{i} \binom{4i+4}{2m+1} = 2^{4i+2}
    \end{align*}
    This completes the proof.
\end{proof}
\begin{proposition}
    For every $i$
    \begin{align*}
        \sum_{k=0}^{4i+3} \rascalNumber{4i+3}{k}{i} &= 2^{4i+2}
    \end{align*}
\end{proposition}
In particular, equation~\eqref{eq:binomial_coefficients_column_sum} assumes the following identity in
row sums of iterated rascal triangles
\begin{align*}
    \sum\limits_{k=0}^n \rascalNumber{n}{k}{i} = \sum_{m=0}^{i} \binom{n+1}{2m+1}
\end{align*}
